Specify more loop patterns: reverse for, interruptible for

kremlib/C.Loops.fst
@@ -4,7 +4,6 @@ module C.Loops
  * higher-order functions and specifications, and extracted, using a
  * meta-theoretic argument, to actual C loops. *)
 
-open FStar.Mul
 open FStar.ST
 open FStar.Buffer
 
@@ -14,6 +13,13 @@ module UInt32 = FStar.UInt32
 
 #set-options "--initial_fuel 0 --max_fuel 0 --z3rlimit 20"
 
+(* To be extracted as:
+  {
+    int i = <start>;
+    for (; i != <finish>; ++i) <f>;
+  }
+  // i need not be in scope after the loop
+*)
 val for:
   start:UInt32.t ->
   finish:UInt32.t{UInt32.v finish >= UInt32.v start} ->
@@ -31,3 +37,82 @@ let rec for start finish inv f =
     f start;
     for (UInt32.(start +^ 1ul)) finish inv f
   end
+
+(* To be extracted as:
+  {
+    int i = <start>;
+    for (; i != <finish>; --i) <f>;
+  }
+  // i need not be in scope after the loop
+*)
+val reverse_for:
+  start:UInt32.t ->
+  finish:UInt32.t{UInt32.v finish <= UInt32.v start} ->
+  inv:(HS.mem -> nat -> Type0) ->
+  f:(i:UInt32.t{UInt32.(v start >= v i /\ v i > v finish)} -> Stack unit
+                        (requires (fun h -> inv h (UInt32.v i)))
+                        (ensures (fun h_1 _ h_2 -> UInt32.(inv h_1 (v i) /\ inv h_2 (v i - 1)))) ) ->
+  Stack unit
+    (requires (fun h -> inv h (UInt32.v start)))
+    (ensures (fun _ _ h_2 -> inv h_2 (UInt32.v finish)))
+let rec reverse_for start finish inv f =
+  if start = finish then
+    ()
+  else begin
+    f start;
+    reverse_for (UInt32.(start -^ 1ul)) finish inv f
+  end
+
+(* To be extracted as:
+    int i = <start>;
+    bool b = false;
+    for (; b || (i != <end>); ++i) {
+      b = <f>;
+    }
+    // i and b must be in scope after the loop
+*)
+val interruptible_for:
+  start:UInt32.t ->
+  finish:UInt32.t{UInt32.v finish >= UInt32.v start} ->
+  inv:(HS.mem -> nat -> bool -> GTot Type0) ->
+  f:(i:UInt32.t{UInt32.(v start <= v i /\ v i < v finish)} -> Stack bool
+                        (requires (fun h -> inv h (UInt32.v i) false))
+                        (ensures (fun h_1 b h_2 -> inv h_1 (UInt32.v i) false /\ inv h_2 UInt32.(v i + 1) b)) ) ->
+  Stack (UInt32.t * bool)
+    (requires (fun h -> inv h (UInt32.v start) false))
+    (ensures (fun _ res h_2 -> let (i, b) = res in ((if b then True else i == finish) /\ inv h_2 (UInt32.v i) b)))
+let rec interruptible_for start finish inv f =
+  if start = finish then
+    (finish, false)
+  else
+    let start' = UInt32.(start +^ 1ul) in
+    if f start
+    then (start', true)
+    else interruptible_for start' finish inv f
+
+(* To be extracted as:
+    int i = <start>;
+    bool b = false;
+    for (; b || (i != <end>); --i) {
+      b = <f>;
+    }
+    // i and b must be in scope after the loop    
+*)
+val interruptible_reverse_for:
+  start:UInt32.t ->
+  finish:UInt32.t{UInt32.v finish <= UInt32.v start} ->
+  inv:(HS.mem -> nat -> bool -> GTot Type0) ->
+  f:(i:UInt32.t{UInt32.(v start >= v i /\ v i > v finish)} -> Stack bool
+                        (requires (fun h -> inv h (UInt32.v i) false))
+                        (ensures (fun h_1 b h_2 -> inv h_1 (UInt32.v i) false /\ inv h_2 UInt32.(v i - 1) b)) ) ->
+  Stack (UInt32.t * bool)
+    (requires (fun h -> inv h (UInt32.v start) false))
+    (ensures (fun _ res h_2 -> let (i, b) = res in ((if b then True else i == finish) /\ inv h_2 (UInt32.v i) b)))
+let rec interruptible_reverse_for start finish inv f =
+  if start = finish then
+    (finish, false)
+  else
+    let start' = UInt32.(start -^ 1ul) in
+    if f start
+    then (start', true)
+    else interruptible_reverse_for start' finish inv f
